\section{Tutorial 2}

\textbf{Problem 1.}
Use the negative binomial theorem and substitutions to give a formula for the
coefficient of $ x^n $ in $ (1-3x)^{-1} + 2(1-2x)^{-2} $.

\textbf{Solution.}
Recall:

\begin{Theorem}{Negative Binomial Theorem}{}
    Let $ m,k\in\mathbb{Z}_{\geqslant 0} $, then
    \[ (1-x)^{-k}=\sum\limits_{m\geqslant 0}\binom{m+k-1}{k-1}x^m \]
\end{Theorem}


\[ (1-3x)^{-1}=\sum\limits_{m\geqslant 0}\binom{m+1-1}{1-1} (3x)^m
    =\sum\limits_{m\geqslant 0} 3^m x^m \]
\[ \implies [x^n](1-3x)^{-1}
    =3^n \]

\[ 2(1-2x)^{-2}=2\sum\limits_{m\geqslant 0}\binom{m+2-1}{2-1}(2x)^m
    =2\sum\limits_{m\geqslant 0} (m+1)2^m x^m   \]
\[ \implies [x^n]2(1-2x)^{-2}
    =2(n+1)2^n=(n+1)2^{n+1} \]

Combining,
\[ [x^n]\left[ (1-3x)^{-1} + 2(1-2x)^{-2} \right]
    =3^n+(n+1) 2^{n+1} \]

\textbf{Problem 2.}
Let $ F(x)=x+x^2+\cdots $ and let $ G(x)=1+3x+2x^2 $. Compute the coefficient
of $ x^n $ in $ G(F(x)) $.

\textbf{Solution.}

\[ G(F(x))=1+3(x+x^2+\cdots)+2(x+x^2+\cdots)^2 \]

\begin{align*}
    3(x+x^2+\cdots)
     & = 3x(1+x+x^2+\cdots)                \\
     & =\frac{3x}{1-x}                     \\
     & = 3x \sum\limits_{m\geqslant 0} x^m
\end{align*}

\begin{align*}
    2(x+x^2+\cdots)^2
     & = 2\left[x(1+x+x^2+\cdots)\right]^2                   \\
     & =2\left( \frac{x}{1-x}  \right)^2                     \\
     & =2x^2(1-x)^{-2}                                       \\
     & =2x^2 \sum\limits_{m\geqslant 0}\binom{m+2-1}{2-1}x^m \\
     & =2x^2 \sum\limits_{m\geqslant 0}(m+1)x^m
\end{align*}

Computing coefficients,
\[ [x^n]1=
    \begin{cases}
        0, & \text{if } n\geqslant 1 \\
        1, & \text{if } n=0
    \end{cases}
\]

\begin{align*}
    [x^n]3(x+x^2+\cdots)
     & = [x^n] 3x \sum\limits_{m\geqslant 0} x^m   \\
     & = [x^{n-1}]3 \sum\limits_{m\geqslant 0} x^m \\
     & = \begin{cases}
        3, & \text{if } n\geqslant 1 \\
        0, & \text{if } n=0
    \end{cases}
\end{align*}

\begin{align*}
    [x^n]2(x+x^2+\cdots)^2
     & = [x^n]2x^2 \sum\limits_{m\geqslant 0}(m+1)x^m \\
     & = [x^{n-2}]2\sum\limits_{m\geqslant 0}(m+1)x^m \\
     & = \begin{cases}
        2n-2, & \text{if } n\geqslant 2 \\
        0,    & \text{if } n\in\{0,1\}
    \end{cases}
\end{align*}

Thus,
\[ [x^n]G(F(x))
    =\begin{cases}
        2n+1, & \text{if }  n\ge 2 \\
        3,    & \text{if } n=1     \\
        1,    & \text{if } n=0
    \end{cases}
\]

\textbf{Problem 3.} Show that if $ F(x)=a_0+a_1x+a_2x^2+\cdots $. Then
\[ F(x)(1-x)=a_0+(a_1-a_0)x+(a_2-a_1)x^2+\cdots \]
and
\[ F(x)(1-x)^{-1}=\sum\limits_{n=0}^{\infty} c_n x^n, \]
where $ c_n=a_0+a_1+\cdots+a_n $.

\textbf{Solution.}

\emph{Part 1.}
\begin{align*}
    F(x)(1-x)
     & =(a_0+a_1x+a_2x^2+\cdots)(1-x)                      \\
     & =a_0 + (a_1-a_0)x+(a_2-a_1)x^2-a_2x^3-a_3x^4+\cdots
\end{align*}
as required.

\emph{Part 2.}

We know that $ (1-x)^{-1}=1+x+x^2+\cdots $, thus
\begin{align*}
    F(x)(1-x)^{-1}
     & = F(x)+xF(x)+x^2F(x)+\cdots                                    \\
     & =\sum\limits_{i\geqslant 0}x^{i} F(x)                          \\
     & =\sum\limits_{i\geqslant 0}[x^{n-i}] F(x)                      \\
     & =\sum\limits_{i= 0}^{n} a_{n-i} \text{ for } 0\leq k=n-i\leq n \\
     & =\sum\limits_{k=0}^{n} a_k
\end{align*}
where
\[ [x^{n-i}]F(x)
    =\begin{cases}
        a_{n-i}, & \text{if } i\leqslant n \\
        0,       & \text{if } i>n
    \end{cases}
\]

\textbf{Problem 4.} Show that for $ k\geqslant 1 $ and $ n\geqslant 1 $, we have
\[ \sum\limits_{i=0}^{k} (-1)^i\binom{k}{i}\binom{n-i+k-1}{k-1}=0, \]
where we interpret $ \binom{j}{i}=0 $ when $ j<i $.
Hint: Look at $ 1=(1-x)^{k}(1-x)^{-k} $ and compute the coefficient of $ x^n $
in both sides.

\textbf{Solution.}

\[ [x^n]1=
    \begin{cases}
        0, & \text{if } n\geqslant 1 \\
        1, & \text{if } n=0
    \end{cases}
\]

\begin{align*}
    (1-x)^{-k}(1-x)^k
     & = \sum\limits_{j\geqslant 0} \sum\limits_{i=0}^{k}
    (-1)^i\binom{k}{i}\binom{j+k-1}{k-1}x^{j+i}\qquad\text{Negative Bin.\ and Bin. Theorem}
\end{align*}
Let $ j+i=n\iff j=n-i $ to compute $ [x^n](1-x)^{-k}(1-x)^k $, and we get
\[ \sum\limits_{i=0}^{k} (-1)^i\binom{k}{i}\binom{n-i+k-1}{k-1}=0 \]
for $ k\geqslant 1 $ and $ n\geqslant 1 $ as desired.
