\subsection{Arithmetic For Limits}
If we can avoid using the definition to find a limit, we should.
There are certain rules we can follow to compute lots of sequence limits.
Let's see them now!
\begin{Theorem}{}{}
    \begin{enumerate}[(1)]
        \item $ \alpha>0\implies \lim\limits_{{n} \to {\infty}}n^\alpha=\infty $.
        \item $ \alpha<0\implies \lim\limits_{{n} \to {\infty}}n^\alpha=0 $.
    \end{enumerate}
\end{Theorem}
\begin{Theorem}{Arithmetic Rules for Limits of Sequences}{}
    Let $ \Set{a_n} $ and $ \Set{b_n} $ be sequences in $ \R $ and let $ c\in\R $.
    Suppose that $ \Set{a_n} $ and $ \Set{b_n} $ both converge with $ a_n\to L $ and $ b_n\to M $. Then
    \begin{enumerate}[(1)]
        \item if $ a_n=C $ for all $ n $, then $ C=L $,
        \item $ \lim\limits_{{n} \to {\infty}}c a_n=cL $,
        \item $ \lim\limits_{{n} \to {\infty}}(a_n+b_n)=L+M $,
        \item $ \lim\limits_{{n} \to {\infty}}(a_n-b_n)=L-M $,
        \item $ \lim\limits_{{n} \to {\infty}}a_n b_n=LM $,
        \item if $ M\ne 0 $, $ \lim\limits_{{n} \to {\infty}}\frac{a_n}{b_n}=\frac{L}{M} $,
        \item for all $ k\in \N $, $ \lim\limits_{{n} \to {\infty}}a_{n+k}=L $.
    \end{enumerate}
    \tcblower{}
    \textbf{Proof}: Exercises, but let's prove (3) as an example.
    Let $ \varepsilon>0 $ be given. Since $ \lim\limits_{{n} \to {\infty}}a_n=L $,
    we can find $ N_1\in \N $ so that if $ n\ge N_1 $,
    we get $ \abs{a_n-L}<\varepsilon/2 $. Also,
    since $ \lim\limits_{{n} \to {\infty}}b_n=M $, we can find $ N_2\in \N $
    so that if $ n\ge N_2 $, we have $ \abs{b_n-M}<\varepsilon/2 $.
    Now, let $ N=\max(N_1,N_2) $. Then, if $ n\ge N $
    we get
    \[ \abs{(a_n+b_n)-(L+M)}\le \abs{a_n-L}+\abs{b_n-M}<\frac{\varepsilon}{2}+\frac{\varepsilon}{2}=\varepsilon, \]
    where we used the triangle inequality in the first inequality.
\end{Theorem}
\begin{Remark}{}{}
    To use any of the above properties, the limits need to exist!
\end{Remark}
\begin{Example}{}{}
    \begin{enumerate}[(1)]
        \item $ \displaystyle \lim\limits_{{n} \to {\infty}}\frac{3n+7}{n+2}
                  =\lim\limits_{{n} \to {\infty}}\frac{3+7/n}{1+2/n}
                  =\frac{\lim\limits_{{n} \to {\infty}}3+\lim\limits_{{n} \to {\infty}}7/n}{\lim\limits_{{n} \to {\infty}}1+\lim\limits_{{n} \to {\infty}}2/n}
                  =\frac{3+0}{1+0}
                  =3 $.
        \item $ \displaystyle
                  \lim\limits_{{n} \to {\infty}}\frac{n^3+n^2+1}{2n^3+7n^2-1}
                  =\lim\limits_{{n} \to {\infty}}\frac{1+1/n+1/n^3}{2+7/n-1/n^3}
                  =\frac{1+0+0}{2+0+0}
                  =\frac{1}{2} $.
        \item $ \displaystyle
                  \lim\limits_{{n} \to {\infty}}\frac{n+1}{n^2+1}
                  =\lim\limits_{{n} \to {\infty}}\frac{1/n+1/n^2}{1+1/n^2}
                  =\frac{0+0}{1+0}
                  =0 $.
    \end{enumerate}
\end{Example}
\begin{Remark}{}{}
    You don't need to write ``arithmetic rules''
    every time, as we \underline{always} use them!
    Just make sure you show your work!
\end{Remark}
\begin{Example}{}{}
    What if in property (5), $ M=0 $? Anything can happen!
    \begin{itemize}
        \item $ \displaystyle \lim\limits_{{n} \to {\infty}}\frac{1/n}{1/n}=1 $
              even though $ 1/n\to 0 $.
        \item $ \displaystyle \lim\limits_{{n} \to {\infty}}\frac{1/n}{1/n^2}=
                  \lim\limits_{{n} \to {\infty}}\frac{n^2}{n}=
                  \lim\limits_{{n} \to {\infty}}n=\infty $.
        \item $ \displaystyle \lim\limits_{{n} \to {\infty}}\frac{1/n^2}{1/n}=
                  \lim\limits_{{n} \to {\infty}}\frac{1}{n}=0 $.
    \end{itemize}
    Hence, we will need to handle these on an individual basis.
\end{Example}
However, there is one thing we can say.

\begin{Theorem}{}{}
    If $ \lim\limits_{{n} \to {\infty}}b_n=0 $
    and $ \lim\limits_{{n} \to {\infty}}\frac{a_n}{b_n} $
    exists, then $ \lim\limits_{{n} \to {\infty}}a_n=0 $.
    \tcblower{}
    \textbf{Proof}: Suppose $ \lim\limits_{{n} \to {\infty}}b_n=0 $,
    and say $ \lim\limits_{{n} \to {\infty}}\frac{a_n}{b_n}=k\in\R $,
    then
    \[ \lim\limits_{{n} \to {\infty}}a_n=
        \lim\limits_{{n} \to {\infty}}\frac{a_n}{b_n}=
        k\cdot 0=0. \]
\end{Theorem}
\begin{Corollary}{}{}
    If $ \lim\limits_{{n} \to {\infty}}b_n=0 $
    and $ \lim\limits_{{n} \to {\infty}}a_n\ne 0 $,
    then $ \lim\limits_{{n} \to {\infty}}\frac{a_n}{b_n} $
    does not exist.
\end{Corollary}
\begin{Example}{}{}
    \[ \lim\limits_{{n} \to {\infty}}\frac{n^3+3n}{n^2+1}=
        \lim\limits_{{n} \to {\infty}}\frac{1+3/n^2}{1/n+1/n^3}. \]
    However, the numerator converges to $ 1 $,
    while the denominator converges to $ 0 $.
    Therefore, the limit does not exist.

    We could also say
    \[ \lim\limits_{{n} \to {\infty}}\frac{n^3+3n}{n^2+1}=\infty, \]
    which means DNE \underline{and} infinitely large!
\end{Example}
Let's compute the limit of any ratios of powers of $ n $.
\begin{Proposition}{}{}
    \begin{align*}
        \lim\limits_{{n} \to {\infty}}\frac{b_0+b_1n+b_2n^2+\cdots+b_j n^j}{c_0+c_1n+c_2n^2+\cdots+c_k n^k}
         & =\lim\limits_{{n} \to {\infty}}\frac{n^j}{n^k}
        \biggl[\frac{\frac{b_0}{n^j}+\frac{b_1}{n^{j-1}}+\cdots+b_j}{
                \frac{c_0}{n^k}+\frac{c_1}{n^{k-1}}+\cdots+c_k
        }\biggr]                                          \\
         & =\begin{cases}
                \frac{b_j}{c_k}, & j=k,                \\
                0,               & j<k,                \\
                \infty,          & j>k\land b_j/c_k>0, \\
                -\infty,         & j>k\land b_k/c_k<0.
            \end{cases}
    \end{align*}
\end{Proposition}
\begin{Example}{}{}
    \begin{itemize}
        \item \[ \lim\limits_{{n} \to {\infty}}\frac{3n+2}{2n-1}=\frac{3}{2}. \]
        \item \[ \lim\limits_{{n} \to {\infty}}\frac{4n^2+5n}{n^3-1}=0. \]
        \item \[ \lim\limits_{{n} \to {\infty}}\frac{7-n^4}{1+n^3}=-\infty. \]
    \end{itemize}
\end{Example}
\begin{Remark}{}{}
    Still show work when writing solutions on a test though (e.g.,
    dividing by highest power of $ n $).
\end{Remark}
\begin{Example}{}{}
    If we have something that ``looks like'' $ \infty-\infty $,
    then multiply by the conjugate!
    \begin{align*}
        \lim\limits_{{n} \to {\infty}}\sqrt{n^2-4}-n
         & =\lim\limits_{{n} \to {\infty}}\sqrt{n^2-4}-n \frac{\sqrt{n^2+4}+n}{\sqrt{n^2+4}+n} \\
         & =\lim\limits_{{n} \to {\infty}}\frac{n^2+4-n^2}{\sqrt{n^2+4}+n}                     \\
         & =\lim\limits_{{n} \to {\infty}}\frac{4}{\sqrt{n^2+4}+n}                             \\
         & =\lim\limits_{{n} \to {\infty}}\frac{4/n}{\sqrt{1+4/n^2}+1}                         \\
         & =\frac{0}{2}                                                                        \\
         & =0.
    \end{align*}
\end{Example}
\subsection*{Recursive Sequence Limits}
We will examine recursive sequences more closely in 1.4,
but for now, if we know a recursive sequence converges,
then we can use rule (7) to find the limit!
\begin{Example}{}{}
    $ a_1=2 $, $ a_{n+1}=\frac{5+a_n}{2} $.
    Suppose we know it has a limit, say $ \lim\limits_{{n} \to {\infty}}a_n=L $.
    Then, using rule (7), we get:
    \[ L=\lim\limits_{{n} \to {\infty}}a_n=
        \lim\limits_{{n} \to {\infty}}a_{n+1}=
        \lim\limits_{{n} \to {\infty}}\frac{5+a_n}{2}=
        \frac{5+L}{2}. \]
    Therefore,
    \[ L=\frac{5+L}{2}\iff 2L=5+L\iff L=5. \]
\end{Example}
\section{Squeeze Theorem}
\begin{Theorem}{Squeeze Theorem}{}
    If $ a_n\le b_n\le c_n $ and $ \lim\limits_{{n} \to {\infty}}a_n=L=\lim\limits_{{n} \to {\infty}}c_n $,
    then $ \lim\limits_{{n} \to {\infty}}b_n=L $.
    \tcblower{}
    \textbf{Proof}: Let $ \varepsilon>0 $ be given.
    Since $ a_n\to L $ and $ c_n\to L $, we can find $ N\in\N $
    such that if $ n\ge N $, then $ a_n\in(L-\varepsilon,L+\varepsilon) $,
    and $ c_n\in(L-\varepsilon,L+\varepsilon) $. Then, for $ n\ge N $,
    \[ L-\varepsilon\le a_n\le b_n\le c_n\le L+\varepsilon, \]
    so $ b_n\in (L-\varepsilon,L+\varepsilon) $, which means
    $ \lim\limits_{{n} \to {\infty}}b_n=L $.
\end{Theorem}
\begin{Remark}{}{}
    The Squeeze Theorem is great for dealing with $ \sin/\cos $
    and $ (-1)^n $.
\end{Remark}
\begin{Example}{}{}
    Compute the following limits.
    \begin{enumerate}[(1)]
        \item $ \lim\limits_{{n} \to {\infty}}\frac{(-1)^n}{n^2+1} $.
        \item $ \lim\limits_{{n} \to {\infty}}\frac{\cos(n^2+7)+7}{n} $.
    \end{enumerate}
    \tcblower{}
    \textbf{Solution}.
    \begin{enumerate}[(1)]
        \item Notice that $ \frac{-1}{n^2+1}\le \frac{(-1)^n}{n^2+1}\le \frac{1}{n^2+1} $
              and $ \lim\limits_{{n} \to {\infty}}\frac{-1}{n^2+1}=0=\lim\limits_{{n} \to {\infty}}\frac{1}{n^2+1} $,
              so $ \lim\limits_{{n} \to {\infty}}\frac{(-1)^n}{n^2+1}=0 $ by the Squeeze Theorem.
        \item Notice that $ \frac{6}{n}\le \frac{\cos(n^2+7)+7}{n}\le \frac{8}{n} $,
              and since $ \lim\limits_{{n} \to {\infty}}\frac{6}{n}=0=\lim\limits_{{n} \to {\infty}}\frac{8}{n} $,
              we get $ \lim\limits_{{n} \to {\infty}}\frac{\cos(n^2+7)+7}{n}=0 $ by the Squeeze Theorem.
    \end{enumerate}
\end{Example}
\section{Monotone Convergence Theorem}
First, we need to some terminology.
\begin{Definition}{}{}
    Let $ S\subseteq \R $. We say that $ \alpha $ is an \textbf{upper bound}
    of $ S $ if $ x\le \alpha $ for all $ x\in S $. We call
    such a set \textbf{bounded above}.

    Similarly, $ \beta $ is a \textbf{lower bound} if $ x\le \beta $
    for all $ x\in S $. In this case, $ S $ is \textbf{bounded below}.

    We call $ S $ \textbf{bounded} if it is bounded both above and
    below. In this case, we could find $ M\in\R $
    such that $ S\subseteq [-M,M] $.
\end{Definition}
\begin{Example}{}{}
    If $ S=(-1,1) $, then $ 7 $ is an upper bound and $ -12 $
    is a lower bound, so $ S $ is bounded. Another example
    is $ S\subseteq[-5,5] $.
\end{Example}
\begin{Definition}{}{}
    Let $ S\subseteq \R $. $ \alpha $ is called the \textbf{least upper bound}
    of $ S $ if:
    \begin{enumerate}[(i)]
        \item $ \alpha $ is an upper bound, and
        \item $ \alpha $ is the smallest, that is, if $ \alpha' $ is another
              upper bound, then $ \alpha'\ge \alpha $.
    \end{enumerate}
    Denote this by $ \alpha=\text{lub}(S) $ or $ \alpha=\sup(S) $.

    Similarly, $ \beta $ is the \textbf{greatest lower bound} if
    \begin{enumerate}[(i)]
        \item $ \beta $ is a lower bound, and
        \item $ \beta $ is the largest, that is, if $ \beta' $
              is another lower bound, then $ \beta'\le \beta $.
    \end{enumerate}
    Denote this by $ \beta=\text{glb}(S) $ or $ \beta=\inf(S) $.
\end{Definition}
\begin{Example}{}{}
    If $ S=(-1,1) $, then $ \inf(S)=-1 $ and $ \sup(S)=1 $.
\end{Example}
\begin{Remark}{}{}
    The $ \inf(S) $ and $ \sup(S) $ may or may not be in $ S $.
    One of the properties (axioms) of $ \R $ guarantees the existence
    of $ \inf $ and $ \sup $. If $ S\subseteq \R $
    is non-empty and bounded above (below), then $ S $ has
    $ \sup $ ($ \inf $).
\end{Remark}
\begin{Definition}{}{}
    We say that a sequence $ \seq $ is:
    \begin{itemize}
        \item \textbf{increasing} if $ a_n<a_{n+1} $,
        \item \textbf{non-decreasing} if $ a_n\le a_{n+1} $,
        \item \textbf{decreasing} if $ a_n>a_{n+1} $,
        \item \textbf{non-increasing} if $ a_n\ge a_{n+1} $,
        \item \textbf{monotonic} if $ \seq $ is either
              non-decreasing or non-increasing.
    \end{itemize}
\end{Definition}
Now, we can state the theorem!
\begin{Theorem}{Monotone Convergence Theorem (MCT)}{}
    Let $ \seq $ be a non-decreasing (non-increasing) sequence.
    \begin{enumerate}[(1)]
        \item If $ \seq $ is bounded above (below), then $ \seq $
              converges to $ L=\lub(\seq) $ ($ L=\glb(\seq) $).
        \item If $ \seq $ is not bounded above (below),
              then $ \seq $ diverges to $ \infty $ ($ -\infty $).
    \end{enumerate}
    \tcblower{}
    \textbf{Proof}: We will prove the non-decreasing/bounded above case,
    the other case is similar. Suppose $ \seq $ is non-decreasing.
    \begin{enumerate}[(1)]
        \item Suppose $ \seq $ is bounded above and let $ L=\lub(\seq) $.
              Let $ \varepsilon>0 $ be given. Then, $ L-\varepsilon<L $,
              which means that $ L-\varepsilon $ is \underline{not}
              an upper bound of $ \seq $ ($ L $ is the \underline{least}
              upper bound). So, there exists $ N\in\N $ so that $ L-\varepsilon<a_N $.
              Then, if $ n\ge N $, we have $ L-\varepsilon<a_N\le a_n $
              since the sequence is non-decreasing. Therefore,
              for $ n\ge N $, $ L-\varepsilon<a_n\le L<L+\varepsilon $,
              so the tail of $ \seq $ is in $ (L-\varepsilon,L+\varepsilon) $,
              which means $ \lim\limits_{{n} \to {\infty}}a_n=L $.
        \item Suppose $ \seq $ is not bounded above. Let $ M\in\R $
              be given. We can find $ N\in\N $ so that $ M<a_N $. Then, if
              $ n\ge N $, we have $ M<a_N<a_n $ ($ \seq $ is non-decreasing).
              This shows $ \lim\limits_{{n} \to {\infty}}a_n=\infty $.
    \end{enumerate}
\end{Theorem}
\subsubsection{Introduction to Mathematical Induction}
Before we can use the MCT, we need to develop one proof technique:
Mathematical Induction (MATH 135 will explore it further).
Induction is a proof technique that allows us to prove an infinite
number of statements. Say we have statements $ P_1,P_2,P_3,\ldots,P_n,\ldots $
for $ n\in \N $. If we can:
\begin{enumerate}[(1)]
    \item Prove $ P_1 $ is true (base case).
    \item Prove: if $ P_k $ is true for some $ k $ (inductive hypothesis),
          then $ P_{k+1} $ is true (inductive step).
\end{enumerate}
Then, we can conclude that $ P_n $ is true for all $ n\in\N $. Think of dominoes!

We will use the MCT and induction to find the limits of recursive sequences.
To do this, we follow these steps:
\begin{enumerate}[(1)]
    \item Prove the sequence is monotonic.
    \item Prove the sequence is bounded (above or below).
    \item Conclude the sequence converges by MCT\@.
    \item Find the limit using an earlier trick:
          \[ \lim\limits_{{n} \to {\infty}}a_n=\lim\limits_{{n} \to {\infty}}a_{n+1}. \]
\end{enumerate}
Note that the order matters! We can't perform step 4 unless we know
that the sequence converges.
\begin{Example}{}{}
    Let $ a_1=1 $, $ a_{n+1}=\frac{3+a_n}{2} $ for $ n\ge 1 $. Prove
    the sequence converges and find its limit.
    \tcblower{}
    \textbf{Solution}.
    \begin{enumerate}[(1)]
        \item Let's check a few terms: $ a_1=1 $, $ a_2=2 $, $ a_3=5/2 $,
              so it looks like the sequence is non-decreasing.

              Claim: $ a_n\le a_{n+1} $ for all $ n\in N $.
              \begin{itemize}
                  \item Base Case: Is $ a_1\le a_2 $? Yes, since $ a_1=1\le 2=a_2 $.
                  \item Inductive Hypothesis: Suppose $ a_k\le a_{k+1} $ for
                        some $ k\ge 1 $.
                  \item Inductive Step: Since $ a_k\le a_{k+1} $, $ 3+a_{k}\le 3+a_{k+1} $,
                        which means
                        \[ \frac{3+a_k}{2}\le \frac{3+a_{k+1}}{2}, \]
                        that is, $ a_{k+1}\le a_{k+2} $.
              \end{itemize}
              Therefore, the sequence is non-decreasing by induction.
        \item What upper bound should we use? Don't try to guess the $ \lub $
              at this point, any upper bound will do!

              Claim: $ a_n\le 5 $ for all $ n\in\N $.
              \begin{itemize}
                  \item Base Case: $ a_1=1\le 5 $.
                  \item Inductive Hypothesis: Suppose $ a_k\le 5 $
                        for some $ k\in\N $.
                  \item Inductive Step: Since $ a_k\le 5 $, $ 3+a_k\le 8 $,
                        so $ \frac{3+a_k}{2}\le 4 $. Therefore, $ a_{k+1}\le 4\le 5 $.
              \end{itemize}
              Therefore, $ a_n\le 5 $ for all $ n\in\N $ by induction,
              so the sequence is bounded above.
        \item Since $ \seq $ is bounded above and non-decreasing,
              we know $ \seq $ converges by MCT\@.
        \item Now, we know a limit exists, say $ L=\lim\limits_{{n} \to {\infty}}a_n $.
              Then,
              \[ L=\lim\limits_{{n} \to {\infty}}a_n=\lim\limits_{{n} \to {\infty}}a_{n+1}
                  =\lim\limits_{{n} \to {\infty}}\frac{3+a_n}{2}=\frac{3+L}{2}. \]
              So,
              \[ L=\frac{3+L}{2}\iff 2L+3L\iff L=3. \]
              Therefore, $ \lim\limits_{{n} \to {\infty}}a_n=3 $.
    \end{enumerate}
\end{Example}
\begin{Example}{}{}
    Let $ a_1=2 $, $ a_{n+1}=7+a_n $ for $ n\ge 1 $. Prove
    the sequence converges and find its limit.
    \tcblower{}
    \textbf{Solution}. Let's check a few terms: $ a_1=2 $, $ a_2=3 $, $ a_3=\sqrt{10} $,
    so it looks like the sequence is non-decreasing. Let's prove
    bounded above and non-decreasing in one step!
    \begin{enumerate}[(1)]
        \item Claim: $ a_n\le a_{n+1}\le 9 $ for all $ n\in \N $.
              \begin{itemize}
                  \item Base Case: $ a_1=2\le 3=a_2 $ and $ a_2=3\le 9 $,
                        so $ a_1\le a_2\le 9 $.
                  \item Inductive Hypothesis: Assume
                        $ a_k\le a_{k+1}\le 9 $ for some $ k\in \N $.
                  \item Inductive Step: Then,
                        \begin{align*}
                             & a_k\le a_{k+1}\le 9                          \\
                             & \implies 7+a_k\le \sqrt{7+a_{k+1}}\le 4\le 9 \\
                             & \implies a_{k+1}\le a_{k+2}\le 9.
                        \end{align*}
              \end{itemize}
              So, by induction $ a_n\le a_{n+1}\le 9 $ for all $ n\in \N $.
        \item The sequence converges by the MCT\@.
        \item Finally, we need to find the limit. Say $ L=\lim\limits_{{n} \to {\infty}}a_n $.
              Then,
              \[ L=\lim\limits_{{n} \to {\infty}}a_{n+1}=\lim\limits_{{n} \to {\infty}}\sqrt{7+a_n}=\sqrt{7+L}; \]
              see A2Q6 for the last equality. So,
              \[ L=\sqrt{7+L}\implies L^2=7+L\implies L^2-L-7=0\implies L=\frac{1\pm \sqrt{29}}{2}. \]
              However, we know $ L=\lub(\seq) $ and $ a_1=2 $. So, $ L\ne \frac{1-\sqrt{29}}{2} $
              since $ \frac{1-\sqrt{29}}{2}<2 $, that is, it isn't even an upper bound. Hence,
              \[ L=\frac{1+\sqrt{29}}{2}. \]
    \end{enumerate}
\end{Example}