\section{Lecture 19*}
\myuline{Example}

Suppose $ X $ has probability function:

\begin{tabular}{| *{6}{>{\centering\arraybackslash}p{1cm} |}}
    \hline
    $x$ & 0 & 1 & 2 & 3 & 4\\
    \hline
    $y$ & 1 & 3 & 5 & 7 & 9\\
    \hline
    $f(x)$ & 0.1 & 0.1 & 0.1 & 0.5 & 0.2\\
    \hline
\end{tabular}

Let $ Y=2X+1 $.

$ E[X]=2.6 $

$ E[X^2]=6.2 $

$ E[Y]=6.2 $

$ E[Y^2]=94.2 $

$ Var(X)=8.2-2.6^2=1.44 $

$ SD(X)=1.2 $

$ Var(Y)=44.2-6.2^=5.76 $

$SD(Y)=2.4$

Now we can verify,
\begin{align*}
    E[Y]&=E[2X+1]\\
    &=2E[X]+1\\
    &=2(2.6)+1\\
    &=6.2
\end{align*}
\[ Var(Y)=2^2 Var(X)=4(1.44)=5.76 \]
\[ SD(Y)=|2|SD(X)=2(1.2)=2.4 \]

Let $ X \thicksim \bin(n,p) $. Find $ E[X] $.
\setcounter{equation}{0}
\begin{align}
    E[X]&=\sum\limits_{\text{all } x}x f(x)\\
    &=\sum\limits_{x=0}^{n}x \binom{n}{x}p^x(1-p)^{n-x}\\
    &=\sum\limits_{x=1}^{n}x \binom{n}{x}p^x(1-p)^{n-x}\\
    &=\sum\limits_{x=1}^{n}x \frac{n!}{x!(n-x)!}p^x(1-p)^{n-x}\\
    &=\sum\limits_{x=1}^{n}x \frac{n!}{x(x-1)!(n-x)!}p^x(1-p)^{n-x}\\
    &=\sum\limits_{x=1}^{n}\frac{n!}{(x-1)!(n-x)!}p^x(1-p)^{n-x}\\
    &=\sum\limits_{x=1}^{n}\frac{n(n-1)!}{(x-1)![(n-1)-(x-1)]!}pp^{x-1}(1-p)^{(n-1)-(x-1)}\\
    &=np(1-p)^{n-1}\sum\limits_{x=1}^{n}\binom{n-1}{x-1}p^{x-1}(1-p)^{-(x-1)}\\
    &=np(1-p)^{n-1}\sum\limits_{x=1}^{n}\binom{n-1}{x-1}\left(\frac{p}{1-p}\right)^{x-1}
\end{align}
From (2) to (3) we used to fact that when $ x=0 $ the value of the expression 
is $ 0 $. Provided that $ x\neq 0 $, we can expand $ x! $ as $ x(x-1)! $ as
seen from (4) to (5). Let $ y=x-1 $, we get
\begin{align}
    E[X]&=np(1-p)^{n-1}\sum\limits_{y=0}^{n}\binom{n-1}{y}\left(\frac{p}{1-p}\right)^{y}\\
    &=np(1-p)^{n-1}\left(1+\frac{p}{1-p}\right)^{n-1}\\
    &=np(1-p)^{n-1}\frac{(1-p+p)^{n-1}}{(1-p)^{n-1}}\\
    &=np
\end{align}
From (10) to (11) we used the Binomial Theorem.

Let $ X \thicksim \poi(\mu) $. Find $ E[X] $.
\setcounter{equation}{0}
\begin{align}
    E[X]&=\sum\limits_{\text{all } x}x f(x)\\
    &=\sum\limits_{x=0}^{\infty} x \frac{e^{-\mu}\mu^x}{x!}\\
    &=\sum\limits_{x=1}^{\infty} x \frac{e^{-\mu}\mu^x}{x(x-1)!}\\
    &=\sum\limits_{x=1}^{\infty} \mu \frac{e^{-\mu}\mu^{x-1}}{(x-1)!}\\
\end{align}
Let $ y=x-1 $, we get
\begin{align}
    E[X]&=\mu e^{-\mu}\sum\limits_{y=0}^{\infty} \frac{\mu^{y}}{y!}\\
    &=\mu e^{-\mu}e^\mu\\
    &=\mu
\end{align}
From (6) to (7) we used the fact that $ e^x=\sum\limits_{y=0}^{\infty}\frac{x^y}{y!} $.

Similarly,
\[ X \thicksim \du[a,b],\, E[X]=\frac{a+b}{2} \]
\[ X \thicksim \hyp(N,r,n),\, E[X]=\frac{nr}{N} \]
\[ X \thicksim \nb(k,p),\,E[X]=\frac{k(1-p)}{p} \]
\[ X \thicksim \geo(p),\,E[X]=\frac{1-p}{p} \]

Let $ X \thicksim \poi(\mu) $. Find $ Var(X) $.

Since there's $ x! $ in the denominator of $ f(x) $, let's find
$ E[X(X-1)] $.
\begin{align*}
    E[X(X-1)]&=\sum\limits_{x=0}^{\infty}x(x-1)\frac{\mu^xe^{-\mu}}{x!}\\
    &=\sum\limits_{x=2}^{\infty}x(x-1)\frac{\mu^xe^{-\mu}}{x(x-1)(x-2)!}\\
    &=\mu^2e^{-\mu}\sum\limits_{x=2}^{\infty} \frac{\mu^{x-2}}{(x-2)!}\\
\end{align*}
Let $ y=x-2 $, we get
\begin{align*}
    E[X(X-1)]&=\mu^2e^{-\mu}\sum\limits_{y=0}^{\infty} \frac{\mu^{y}}{y!}\\
    &=\mu^2
\end{align*}
\begin{align*}
    Var(X)&=E[X(X-1)]+E[X]-E[X]^2\\
    &=\mu^2+\mu-\mu^2\\
    &=\mu
\end{align*}

