\section{2019-10-07}
\textbf{Directional Derivative}
Recall
\[ \frac{\partial f}{\partial x} =\lim\limits_{{h} \to {0}} 
\frac{f(a+h,b)-f(a,b)}{h} \]
rate of change of $ f $ in the direction $ x=a $.

Choose a direction $ \bm{\hat{u}}=(u_1,u_2) $
\begin{figure}[ht]
    \centering
    \includesvg{./figures/directional}
\end{figure}

$ (x,y)=(a,b)+s(u_1,u_2) $
similar equation for tangent line

when
$ s=0\implies (x,y)=(a,b) $

Consider distance 
\[ ||\bm{x}-\bm{a}||
=||s(u_1,u_2)||=|s|||(u_1,u_2)|| \]
If we choose $ ||\bm{u}||=1 $, then $ |s| $ is the
distance along this from some $ (x,y) $ to
$ (a,b) $.
So, $ ||\bm{u}||=1 $ is a convention.
If $ ||\bm{u}||\neq 1 $, normalize it
\[ \bm{u}=\frac{1}{||\bm{u}||}\bm{u} \]

\begin{thmbox}
    Rate of change of $\bm{u}$ is

    \[ \frac{\partial f}{\partial \bm{u}}(a,b) =
    \lim\limits_{{s} \to {0}}
    \frac{f(a+su_1,b+su_2)-f(a,b)}{s} \]

\end{thmbox}

Other ways to write
\[ \frac{\partial f}{\partial \bm{u}}(a,b) = 
D_{\bm{u}}f(\bm{a})=\frac{d}{ds}f(\bm{a}+s
\bm{u})\Bigr\rvert_{s=0} \]
sub for $ x=a+su_1, y=b+su_2 $
then $ f(x,y) =f(a+su_1,b+su_2)=f(\bm{a}+s\bm{u})$