\chapter{Techniques of Integration}
\section{Trigonometric Substitution}
Sometimes, changing $ x $ into a trigonometric function can
simplify an integral!

There are three situations where this is useful: say $ \alpha\in\mathbb{R} $.

\begin{table}[!htbp]
    \centering
    \begin{tabular}{ccc}
        If you see:        & Try substituting:   & Range for $ \theta $                                                         \\
        \midrule
        $ \sqrt{a^2-x^2} $ & $ x=a\sin(\theta) $ & $ \theta\in\interval[open]{-\sfrac{\pi}{2}}{\sfrac{\pi}{2}} $                \\
        $ \sqrt{a^2+x^2} $ & $ x=a\tan(\theta) $ & $ \theta\in\interval[open]{-\sfrac{\pi}{2}}{\sfrac{\pi}{2}} $                \\
        $ \sqrt{x^2-a^2} $ & $ x=a\sec(\theta) $ & $ \theta\in\interval{0}{\sfrac{\pi}{2}}\cup\interval{\pi}{\sfrac{3\pi}{2}} $
    \end{tabular}
\end{table}

\begin{Remark}{}{}
    \begin{itemize}
        \item The range for $ \theta $ is important to ensure that
              $ \sin(\theta)/\tan(\theta)/\sec(\theta) $ are invertible (so we can
              solve for $ \theta $ in terms of $ x $, if need be).
        \item No, you don't need to state the range for $ \theta $ each time.
        \item The integrand may need to be simplified before a trigonometric substitution
              can be made.
        \item Don't forget to change back to $ x $ in an indefinite integral.
    \end{itemize}
\end{Remark}

\begin{Example}{}{}
    Compute $ \displaystyle   \int \frac{1}{\sqrt{x^2+4}} \odif{x} $.

    \textbf{Solution.}
    \begin{align*}
        \int \frac{1}{\sqrt{x^2+4}} \odif{x}
         & =\int \frac{1}{\sqrt{4\tan^2(\theta)+4}} \left(2\sec^2(\theta)\right) \odif{\theta}
         &                                                                                     & x=2\tan(\theta)\iff \odif{x}=2\sec^2(\theta)\odif{\theta}                               \\
         & =\int \frac{\sec^2(\theta)}{\sqrt{\tan^2(\theta)+1}} \odif{\theta}                                                                                                            \\
         & =\int \frac{\sec^2(\theta)}{\sqrt{\sec^2(\theta)}} \odif{\theta}                                                                                                              \\
         & =\int \frac{\sec^2(\theta)}{\abs{\sec(\theta)}} \odif{\theta}                                                                                                                 \\
         & =\int \sec(\theta)\odif{\theta}                                                     &                                                           & \text{since }\sec(\theta)>0 \\
         & =\ln\abs{\sec{\theta}+\tan(\theta)}+C                                               &                                                                                         \\
         & =\ln\abs*{\frac{\sqrt{x^2+4}}{2}+\frac{x}{2}}+C
    \end{align*}
    where we substituted $
        \displaystyle x=2\tan(\theta)\iff \tan(\theta)=\frac{x}{2}\implies
        \sec(\theta)=\frac{\sqrt{x^2+4}}{2} $ in the last step (try to visualize a triangle).
\end{Example}

\begin{Remark}{}{}
    When using a trigonometric substitution, the absolute values will \textbf{always}
    go away due to the choice of $ \theta $'s!
\end{Remark}

\begin{Example}{}{}
    \begin{enumerate}[label=(\roman*)]
        \item Compute $ \displaystyle \int \frac{\sqrt{9-4x^2}}{x^2} \odif{x} $.

              \textbf{Solution.}
              \begin{align*}
                  \int \frac{\sqrt{9-4x^2}}{x^2} \odif{x}
                   & =2 \int \frac{\sqrt{\sfrac{9}{4}-x^2}}{x^2} \odif{x}                                                                                                                                                                              \\
                   & =2 \int \frac{\sqrt{\sfrac{9}{4}-\sfrac{9}{4}\sin^2(\theta)}\left( \sfrac{3}{2}\cos(\theta) \right)}{\sfrac{9}{4}\sin^2(\theta)} \odif{\theta} &  & x=\sfrac{3}{2}\sin(\theta)\iff \odif{x}=\sfrac{3}{2}\cos(\theta)\odif{\theta} \\
                   & =2 \frac{3}{2} \cdot \frac{3}{2} \cdot \frac{4}{9}
                  \int \frac{\sqrt{1-\sin^2(\theta)}\cos(\theta)}{\sin^2(\theta)} \odif{\theta}                                                                                                                                                        \\
                   & =2 \int \frac{\abs{\cos(\theta)}\cos(\theta)}{\sin^2(\theta)} \odif{\theta}                                                                                                                                                       \\
                   & =2 \int \frac{\cos^2(\theta)}{\sin^2(\theta)} \odif{\theta}                                                                                    &  & \text{since }\cos(\theta)>0                                                   \\
                   & =2 \int \cot^2(\theta)\odif{\theta}                                                                                                                                                                                               \\
                   & =2 \int \csc^2(\theta)-1\odif{\theta}                                                                                                                                                                                             \\
                   & =2[-\cot(\theta)-\theta]+C                                                                                                                                                                                                        \\
                   & =2\left[ -\frac{\sqrt{9-4x^2}}{2x}-\arcsin\left( \frac{2x}{3} \right) \right]+C
              \end{align*}
              Where we substituted $ \displaystyle
                  x=\frac{3}{2}\sin(\theta)\iff \frac{2x}{3}=\sin(\theta)\implies
                  \theta=\arcsin\left( \frac{2x}{3} \right) $ and $
                  \displaystyle \cot(\theta)=
                  \frac{\sqrt{9-4x^2}}{2x} $ in the last step.
        \item Compute $ \displaystyle \int \frac{1}{x^2\sqrt{x^2-4}} \odif{x} $.

              \textbf{Solution.}
              \begin{align*}
                  \int \frac{1}{x^2\sqrt{x^2-4}} \odif{x}
                   & =\int \frac{2\sec(\theta)\tan(\theta)}{4\sec^2(\theta)\sqrt{4\sec^2(\theta)-4}} \odif{\theta} &  & x=2\sec(\theta)\iff \odif{x}=2\sec(\theta)\tan(\theta)\odif{\theta} \\
                   & =\frac{1}{4} \int \frac{\tan(\theta)}{\sec(\theta)\sqrt{\sec^2(\theta)-1}}\odif{\theta}                                                                                \\
                   & =\frac{1}{4} \int \frac{\tan(\theta)}{\sec(\theta)\tan(\theta)} \odif{\theta}                                                                                          \\
                   & =\frac{1}{4} \int \frac{\tan(\theta)}{\sec(\theta)+\tan(\theta)} \odif{\theta}                                                                                         \\
                   & =\frac{1}{4} \int \frac{1}{\sec(\theta)} \odif{\theta}                                                                                                                 \\
                   & =\frac{1}{4} \int \cos(\theta)\odif{\theta}                                                                                                                            \\
                   & =\frac{\sin(\theta)}{4} +C                                                                                                                                             \\
                   & =\frac{\sqrt{x^2-4}}{4x} +C
              \end{align*}
              Where we substituted $ \displaystyle x=2\sec(\theta)\implies \sin(\theta)=\frac{\sqrt{x^2-4}}{x} $
              in the last step.
        \item Compute $ \displaystyle \int x\sqrt{x^2-9}\odif{x} $.

              \textbf{Solution.}
              \begin{align*}
                  \int x\sqrt{x^2-9}\odif{x}
                   & =\int \frac{x\sqrt{u}}{2x} \odif{u}                        &  & u=x^2-9\iff \odif{u}=2x\odif{x} \\
                   & =\frac{1}{2} \int \sqrt{u}\odif{u}                                                              \\
                   & =\frac{1}{2} \left( \frac{2}{3} \right) u^{\sfrac{3}{2}}+C                                      \\
                   & =\frac{1}{3}\left( x^2-9 \right)^{\sfrac{3}{2}}+C
              \end{align*}
        \item Compute $ \displaystyle  \int_{0}^{3} \frac{x}{(1+x^2)^2} \odif{x} $.

              \textbf{Solution.}
              \begin{align*}
                  \int_{0}^{\sqrt{3}} \frac{x}{(1+x^2)^2} \odif{x}
                   & =\int_{0}^{\sfrac{\pi}{3}}
                  \frac{\tan(\theta)\sec^2(\theta)}{\left[ 1+\tan^2(\theta) \right]^2} \odif{\theta}
                   &                                                                                                         & x=\tan(\theta)\iff \odif{x}=\sec^2(\theta)\odif{\theta}                                                         \\
                   & =\int_{0}^{\sfrac{\pi}{3}} \frac{\tan(\theta)\sec^2(\theta)}{\sec^4(\theta)} \odif{\theta}                                                                                                                                \\
                   & =\int_{0}^{\sfrac{\pi}{3}} \frac{\tan(\theta)}{\sec^2(\theta)} \odif{\theta}                                                                                                                                              \\
                   & =\int_{0}^{\sfrac{\pi}{3}} \frac{\sin(\theta)}{\cos(\theta)} \left( \cos^2(\theta) \right)\odif{\theta}                                                                                                                   \\
                   & =\int_{0}^{\sfrac{\pi}{3}}\sin(\theta)\cos(\theta)\odif{\theta}                                         &                                                         & u=\sin(\theta)\iff \odif{u}=\cos(\theta)\odif{\theta} \\
                   & =\int_{0}^{\sfrac{\sqrt{3}}{2}} u\odif{u}                                                                                                                                                                                 \\
                   & =\left[\frac{u^2}{2} \right]^{\sfrac{\sqrt{3}}{2}}_0                                                                                                                                                                      \\
                   & =\frac{3}{4}
              \end{align*}
    \end{enumerate}
\end{Example}
\begin{Remark}{}{}
    You may need to complete the square before making a trigonometric substitution.
\end{Remark}
\begin{Exercise}{}{}
    Show that $ 3-2x-x^2=4-(x+1)^2 $ by completing the square.
\end{Exercise}
\begin{Example}{}{}
    Compute $ \displaystyle \int \frac{x}{(3-2x-x^2)^{\sfrac{3}{2}}} \odif{x} $.

    \textbf{Solution.}
    Substitution: $ x+1=2\sin(\theta)\iff \odif{x}=2\cos(\theta)\odif{\theta} $.
    \begin{align*}
        \int \frac{x}{(3-2x-x^2)^{\sfrac{3}{2}}} \odif{x}
         & =\int \frac{x}{\left[ 4-(x+1)^2 \right]^{\sfrac{3}{2}}} \odif{x}                                                                \\
         & =\int \frac{[2\sin(\theta)-1] (2\cos(\theta))}{\left[4-4\sin^2(\theta)\right]^{\sfrac{3}{2}}} \odif{\theta}                     \\
         & =\frac{1}{4} \int \frac{[2\sin(\theta)-1]\left(\cos(\theta)\right)}{\left[ \cos^2(\theta) \right]^{\sfrac{3}{2}}} \odif{\theta} \\
         & = \frac{1}{4} \int \frac{2\sin(\theta)-1}{\cos^2(\theta)} \odif{\theta}                                                         \\
         & =\frac{1}{4} \int \frac{2\sin(\theta)}{\cos^2(\theta)}-\frac{1}{\cos^2(\theta)} \odif{\theta}                                   \\
         & =\frac{1}{4} \int 2\tan(\theta)\sec(\theta)-\sec^2(\theta)\odif{\theta}                                                         \\
         & =\frac{1}{4} \left[ 2\sec(\theta)-\tan(\theta) \right]+C                                                                        \\
         & =\frac{1}{4} \left[ \frac{4}{\sqrt{4-(x+1)^2}}-\frac{(x+1)}{\sqrt{4-(x+1)^2}} \right]+C
    \end{align*}
    Where we substituted $ \displaystyle
        x+1=2\sin(\theta)\iff \sin(\theta)=\frac{x+1}{2}\implies
        \sec(\theta)=\frac{2}{\sqrt{4-(x+1)^2}} $ and $
        \displaystyle \tan(\theta)=\frac{x+1}{\sqrt{4-(x+1)^2}} $
    in the last step.
\end{Example}

\section{Integration by Parts}
Let $ u $ and $ v $ be functions of $ x $. From the product rule, we know
\[ \odv{}{x}[uv]=u \odv{v}{x}+v \odv{u}{x} \]
Integrating both sides gives:
\[ \int \odv{}{x} [uv]\odif{x}=\int u \odv{v}{x} \odif{x}+
    \int v \odv{u}{x} \odif{x}   \]
Omit $ \odif{x} $'s to make
\[ uv=\int u\odif{v} -\int v\odif{u} \]
So, we get:
\[ \boxed{\int u\odif{v} =uv-\int v\odif{u}} \]
Strategy: When integrating the product of two functions, pick one to
integrate (call it $ \odif{v} $), and one to differentiate (call it $ u $).
\begin{itemize}
    \item Pick $ \odif{v} $ to be the most difficult function you know how to integrate.
    \item Pick $ u $ so that it gets simpler when differentiated.
\end{itemize}
Or, use ILATE\@: Pick $ u= $ the first function in the list:
\begin{itemize}
    \item I\@: Inverse trigonometric functions
    \item L\@: Logarithmic functions
    \item A\@: Algebraic functions (powers of $ x $)
    \item T\@: Trigonometric functions
    \item E\@: Exponential functions
\end{itemize}

\begin{Example}{}{}
    \begin{enumerate}[label=(\roman*)]
        \item Compute $ \displaystyle \int x^2\ln(x)\odif{x}  $.

              \textbf{Solution.} Let $ u=\ln(x) $ and $ \odif{v}=x^2\odif{x} $, so we have
              $ \odif{u}=\dfrac{1}{x} \odif{x} $ and $ v=\dfrac{x^3}{3} $.
              \begin{align*}
                  \int x^2\ln(x)\odif{x}
                   & =\frac{x^3}{3} \ln(x)-\int \frac{x^3}{3} \left( \frac{1}{x} \right) \odif{x} \\
                   & =\frac{x^3}{3} \ln(x)-\int \frac{x^2}{3}\odif{x}                             \\
                   & =\frac{x^3}{3} \ln(x)-\frac{x^3}{9} +C
              \end{align*}
        \item Compute $ \displaystyle \int x e^x\odif{x} $.

              \textbf{Solution.} Let $ u=x $ and $ \odif{v}=e^x\odif{x} $, so we have $ \odif{u}=\odif{x} $ and $ v=e^x $.
              \[
                  \int x e^x\odif{x}
                  =x e^x-\int e^x\odif{x}
                  =x e^x-e^x+C
              \]
        \item Compute $ \displaystyle \int_{0}^{\pi} x\cos(x)\odif{x} $.

              \textbf{Solution.} Let $ u=x $ and $ \odif{v}=\cos(x)\odif{x} $, so we have $ \odif{u}=\odif{x} $ and $ v=\sin(x) $.
              \[
                  \int_{0}^{\pi} x\cos(x)\odif{x}
                  =\bigl[x\sin(x)\bigr]^{\pi}_{0}-\int_{0}^{\pi} \sin(x)\odif{x}
                  =\bigl[\cos(x)\bigr]^{\pi}_{0}
                  =\cos(\pi)-\cos(0)
                  =-1-1
                  =-2
              \]
        \item Compute $ \displaystyle \int \ln(x)\odif{x} $.

              \textbf{Solution.} Sometimes, we don't want to integrate any part! Let $ u=\ln(x) $
              and $ \odif{v}=\odif{x} $, so we have $ \odif{u}=\dfrac{1}{x}\odif{x} $ and $ v=x $.
              \[
                  \int \ln(x)\odif{x}
                  =x\ln(x)-\int \frac{x}{x} \odif{x}
                  =x\ln(x)-x+C
              \]
              This method also works for $ \int \arctan(x)\odif{x} $ and
              $ \int \arccos(x)\odif{x} $, etc.
        \item Compute $ \displaystyle  \int x^2\cos(x)\odif{x} $.

              \textbf{Solution.} We may need to apply it more than once! Let $ u=x^2 $ and $ \odif{v}=\cos(x)\odif{x} $,
              so we have $ \odif{u}=2x\odif{x} $ and $ v=\sin(x) $.
              \[
                  \int x^2\cos(x)\odif{x}
                  =x^2\sin(x)-\int 2x\sin(x)\odif{x}
              \]
              Let $ u=2x $ and $ \odif{v}=\sin(x)\odif{x} $, so we have $ \odif{u}=2\odif{x} $ and $ v=-\cos(x) $.
              \begin{align*}
                   & =x^2\sin(x)-\left[-2x\cos(x)-\int -2\cos(x)\odif{x} \right] \\
                   & =x^2\sin(x)+2x\cos(x)-\int 2\cos(x)\odif{x}                 \\
                   & =x^2\sin(x)+2x\cos(x)-2\sin(x)+C
              \end{align*}
        \item Compute $ \displaystyle \int e^x\cos(x)\odif{x} $.

              \textbf{Solution.} And sometimes, we don't integrate at all! Let $ u=\cos(x) $
              and $ \odif{v}=e^x\odif{x} $, so we have $ \odif{u}=-\sin(x)\odif{x} $ and $ v=e^x $.
              \[
                  I =\int e^x\cos(x)\odif{x}
                  =e^x\cos(x)+\int e^x\sin(x)\odif{x}
              \]
              Let $ u=\sin(x) $ and $ \odif{v}=e^x\odif{x} $, so we have $ \odif{u}=\cos(x)\odif{x} $ and $ v=e^x $.
              \[
                  I=e^x\cos(x)+e^x\sin(x)-\int e^x\cos(x)\odif{x}
                  =e^x\cos(x)+e^x\sin(x)-I
              \]
              So, $ 2I=e^x\cos(x)+e^x\sin(x) $, therefore
              \[ I=\frac{e^x\cos(x)+e^x\sin(x)}{2} +C \]
              Neat!
        \item Compute $ \displaystyle \int x^3\cos(x^2)\odif{x} $.

              \textbf{Solution.} Sometimes, a combination of methods is needed.
              \begin{align*}
                  \int x^3\cos(x^2)\odif{x}
                   & =\int x^2\cos(u)\frac{1}{2x} \odif{u} &  & u=x^2\iff \odif{u}=2x\odif{x} \\
                   & =\frac{1}{2} \int x^2\cos(u)\odif{u}                                     \\
                   & =\frac{1}{2} \int u\cos(u)\odif{u}                                       \\
              \end{align*}
              Now, do integration by parts with some unfortunate (but fine) letter
              choices! Let $ u=u $ and $ \odif{v}=\cos(u)\,\odif{u} $, so we have $ \odif{u}=\odif{u} $
              and $ v=\sin(u) $.
              \begin{align*}
                   & =\frac{1}{2} u\sin(u)-\frac{1}{2} \int \sin(u)\odif{u} \\
                   & =\frac{1}{2} u\sin(u)+\frac{1}{2} \cos(u)+C            \\
                   & =\frac{1}{2} x^2\sin(x^2)+\frac{1}{2} \cos(x^2)+C
              \end{align*}
    \end{enumerate}
\end{Example}

\section{Partial Fractions}
Partial fractions are useful for evaluating $ \displaystyle \int \frac{p(x)}{q(x)} \odif{x} $
where $ p $ and $ q $ are polynomials.

Overall idea: break a difficult integrand into many easy ones!
\begin{Remark}{}{}
    We will assume the degree of the denominator is \textbf{larger} than the
    degree of the numerator. If not, use long division first!
\end{Remark}

\begin{table}[!htbp]
    \centering
    \caption{How to Break up Fractions: The Rules}
    \begin{tabular}{cc}
        \toprule
        If the denominator has:                      & Then we write:                      \\
        \midrule
        (I) Distinct linear factors                  & One constant per factor             \\
        (II) A repeated linear factor                & One constant per power              \\
        (III) Distinct irreducible quadratic factors & One \textbf{linear term} per factor \\
        (IV) Repeated irreducible quadratic factors  & One linear term per power
    \end{tabular}
\end{table}

\begin{Example}{Decomposition Practice}{}
    \begin{enumerate}[label=(\roman*)]
        \item $ \displaystyle \frac{1}{(x+1)(x+2)}=\frac{A}{x+1}+\frac{B}{x+2} $
        \item $ \displaystyle \frac{1}{x^2(x-1)}=\frac{A}{x} +\frac{B}{x^2}+\frac{C}{x-1} $
        \item $ \displaystyle \frac{x^3+x+7}{x^2(x+1)^2(x^2+1)}=\frac{A}{x} +\frac{B}{x^2}+\frac{C}{x+1}
                  +\frac{D}{(x+1)^2}+\frac{Ex+F}{x^2+1} $
        \item $ \displaystyle \frac{x^2+7}{(x-1)^3(x^2+3)^2}
                  =\frac{A}{x-1} +\frac{B}{(x-1)^2}+\frac{C}{(x-1)^3}+\frac{Dx+E}{x^2+3}
                  +\frac{Fx+G}{(x^2+3)^3} $
        \item $ \displaystyle \frac{x^{10}+5}{(x+1)^3(x^2+1)}=\cdots\text{use long division first, not partial
                      fractions} $
    \end{enumerate}
\end{Example}

\begin{Remark}{What integrals could we be left with after partial fractions?}{}

    \underline{Case 1}: $ \displaystyle \int \frac{A}{ax+b} \odif{x} =\frac{A}{a}\ln\abs{ax+b}+C $

    \underline{Case 2}: $ \displaystyle \int \frac{A}{(ax+b)^n} \odif{x} =\left( \frac{A}{a} \right) \frac{(ax+b)^{-n+1}}{-n+1} $
    where $ n\neq 0,1 $.

    \underline{Case 3}: $ \displaystyle \frac{Ax+B}{ax^2+bx+c} =\int \frac{Ax}{ax^2+bx+c} +\frac{B}{ax^2+bx+c} \odif{x}  $

    \underline{Case 4}: $ \displaystyle \frac{Ax+B}{\left( ax^2+bx+c \right)^n} $

    Note for Case 3 and Case 4, you may want to complete the square and use a trigonometric
    substitution. A regular substitution may also work.
\end{Remark}

\begin{Example}{Partial Fractions (Easy)}{}
    Using partial fractions, compute
    $ \displaystyle \int \frac{x}{x^2-4x-5} \odif{x} $.

    \textbf{Solution.}
    First, we break it up with partial fractions.
    \[ \frac{x}{x^2-4x-5} =\frac{x}{(x+1)(x-5)}=\frac{A}{x+1} +\frac{B}{x-5} \]
    Multiply both sides by the LHS denominator to get the following.
    \begin{align*}
        x & =(x+1)(x-5)\left[ \frac{A}{x+1} +\frac{B}{x-5}  \right] \\
        x & =A(x-5)+B(x+1)
    \end{align*}
    There are two ways we can solve for $ A $ and $ B $.
    \begin{enumerate}[label=(\roman*)]
        \item Linear Algebra!
              \[ x=Ax-5A+Bx+B=(A+B)x+(-5A+B) \]
              Therefore, $ A+B = 1 $ and $ B-5A=0 $. Thus, $ A=\sfrac{1}{6} $
              and $ B=\sfrac{5}{6} $.
        \item Substitute in ``nice'' values for $ x $.
              \begin{align*}
                  x & =5\colon \quad 5   =A(0)+B(6)  \\
                  x & =1\colon \quad -1  =A(-6)+B(0)
              \end{align*}
              Thus, $ A=\sfrac{1}{6} $ and $ B=\sfrac{5}{6} $.
    \end{enumerate}
    Either way, we get
    \[ \frac{x}{(x+1)(x-5)}=\frac{\sfrac{1}{6}}{x+1}+\frac{\sfrac{5}{6}}{x-5}  \]
    So,
    \[
        \int \frac{x}{x^2-4x-5}\odif{x}
        =\frac{1}{6} \int \frac{1}{x+1}\odif{x} +\frac{5}{6} \int \frac{1}{x-5} \odif{x}
        =\frac{1}{6} \ln\abs{x+1}+\frac{5}{6} \ln\abs{x-5}+C
    \]
\end{Example}

\begin{Example}{Partial Fractions (Slightly Difficult)}{}
    Using partial fractions, compute $ \displaystyle \int \frac{x+3}{x^4+9x^2} \odif{x} $.

    \textbf{Solution.}
    First, we break it up with partial fractions.
    \[ \frac{x+3}{x^4+9x^2} =\frac{x+3}{x^2(x^2+9)}=\frac{A}{x}+\frac{B}{x^2} +\frac{Cx+D}{x^2+9}  \]
    Multiply both sides by $ x^2(x^2+9) $ to get the following.
    \begin{align*}
        x+3 & =x(x^2+9)A+(x^2+9)B+x^2(Cx+D) \\
        x+3 & =Ax^3+9Ax+Bx^2+9B+Cx^3+Dx^2   \\
        x+3 & =(A+C)x^3+(B+D)x^2+9Ax+9B
    \end{align*}
    Therefore, $ A+C=0 $, $ B+D=0 $, $ 9A=1 $, and $ 9B=3 $. Thus,
    $ A=\sfrac{1}{9} $, $ B=\sfrac{1}{3} $, $ C=-\sfrac{1}{9} $,
    and $ D=-\sfrac{1}{3} $. So,
    \begin{align*}
        \int \frac{x+3}{x^4+9x^2} \odif{x}
         & =\frac{1}{9} \int \frac{1}{x} \odif{x} +\frac{1}{3} \int \frac{1}{x^2} \odif{x}
        -\frac{1}{9} \int \frac{x}{x^2+9} \odif{x} -\frac{1}{3} \int \frac{1}{x^2+9} \odif{x} \\
         & =\frac{1}{9}\ln\abs{x}-\frac{1}{3x}-\frac{1}{9} \int \frac{x}{x^2+9}\odif{x}
        -\frac{1}{3} \left[ \frac{1}{3}\arctan\left( \frac{x}{3}  \right) \right]             \\
    \end{align*}
    where we computed $ \displaystyle \int \frac{1}{x^2+9}\odif{x} $ with~\ref{remark:arctan_identity}.

    For $ \displaystyle \int \frac{x}{x^2+9} \odif{x}  $, use a substitution: $ u=x^2+9\iff \odif{u}=2x\odif{x} $.
    \[
        \int \frac{x}{x^2+9} \odif{x}
        =\int \frac{x}{u} \frac{1}{2x} \odif{u}
        =\frac{1}{2} \int \frac{1}{u} \odif{u}
        =\frac{\ln\abs{u}}{2} +C
        =\frac{\ln\abs*{x^2+9}}{2} +C
    \]
    So, the final answer is:
    \[ \frac{1}{9}\ln\abs{x}-\frac{1}{3x}-\frac{1}{18}\ln\abs*{x^2+9}
        -\frac{1}{9} \arctan\left( \frac{x}{3}  \right)+C \]
\end{Example}

\begin{Remark}{Useful Identity}{arctan_identity}
    \[ \int \frac{1}{x^2+k^2} \odif{x}=\frac{1}{k} \arctan\left( \frac{x}{k}  \right)+C  \]
\end{Remark}

\begin{Example}{Partial Fractions (Long Division)}{}
    Compute $ \displaystyle \int \frac{x^3-2x}{x^2+3x+2} \odif{x} $.

    \textbf{Solution.}
    Using long division, we get
    \[ \int x-3+\frac{5x+6}{x^2+3x+2} \odif{x}  \]
    Now,
    \[ \frac{5x+6}{x^2+3x+2} =\frac{5x+6}{(x+1)(x+2)} =\frac{A}{x+1} +\frac{B}{x+2} \]
    Therefore, $ 5x+6=A(x+2)+B(x+1) = x(A+B)+(2A+B)$. By inspection,
    we get $ B=4 $ and $ A=1 $. Thus, the integral is:
    \[ \int x-3+\frac{1}{x+1} +\frac{4}{x+2} \odif{x} =\frac{x^2}{2} -3x+\ln\abs{x+1}
        +4\ln\abs{x+2}+C \]
\end{Example}
