\makeheading{Lecture 19 | 2020-11-15}
\section{Some Useful Limit Theorems}
In this section, we'll discuss some theorems
regarding convergence in distribution of $ \bar{X}_n $
or function of $ \bar{X}_n $.
\begin{Theorem}{Central Limit Theorem (CLT)}{}
    Let $ X_1,\ldots,X_n $
    be i.i.d.\ random variables with $ \E{X_i}=\mu $
    and $ \Var{X_i}=\sigma^2<\infty $. Let
    $ \bar{X}=\frac{1}{n} \sum_{i=1}^{n} X_i $. Then,
    the limiting distribution of
    \[ \frac{\sqrt{n}(\bar{X}_n-\mu)}{\sigma} \]
    is the c.d.f.\ of $ \N{0,1} $.
    \[  \frac{\sqrt{n}(\bar{X}_n-\mu)}{\sigma}
        \stackrel{\text{d}}{\to}\N{0,1} \]
\end{Theorem}
The proof is not hard, we use a standard method,
but we need to put several pieces together.
We need the following theorem.
\begin{Theorem}{}{}
    Let $ X_1,\ldots,X_n $ be a sequence of
    random variables such that $ X_n $ has
    m.g.f.\ $ M_n(t) $. Let $ X $
    be another random variable with m.g.f.\
    $ M(t) $. If there exists some $ h>0 $, such that
    \[ \lim\limits_{{n} \to {\infty}} M_n(t)=M(t) \]
    for all $ t\in(-h,h) $, then
    \[ X_n \stackrel{\text{d}}{\to} X \]
\end{Theorem}
Therefore, our next steps:
\begin{enumerate}[label=(\arabic*)]
    \item Find the m.g.f.\ of
          $ \frac{\sqrt{n}(\bar{X}_n-\mu)}{\sigma} $: $ M_n(t) $,
          and m.g.f.\ of $ \N{0,1} $: $ M(t)=e^{t^2/2} $.
    \item We try to show that
          \[ \lim\limits_{{n} \to {\infty}}M_n(t)=e^{t^2/2}  \]
          or
          \[ \lim\limits_{{n} \to {\infty}} \ln{M_n(t)}=\frac{t^2}{2} \]
          for $ t\in(-h,h) $ where $ h>0 $.
\end{enumerate}
Step 1: Find m.g.f.\ of $ \displaystyle \frac{\sqrt{n}(\bar{X}_n-\mu)}{\sigma} $.
\begin{align*}
    \frac{\sqrt{n}(\bar{X}_n-\mu)}{\sigma}
     & =\sqrt{n}\frac{\frac{1}{n} \sum_{i=1}^{n} (X_i-\mu)}{\sigma} \\
     & =\frac{1}{\sqrt{n}} \frac{\sum_{i=1}^{n} (X_i-\mu)}{\sigma}
\end{align*}
Let $ \displaystyle Y_i=\frac{X_i-\mu}{\sigma} $, then
$ Y_1,\ldots,Y_n $ are i.i.d.\ with $ \E{Y_i}=0 $
and $ \Var{Y_i}=1 $. Then,
\begin{align*}
    M_n(t)
     & =\E*{e^{(t)\frac{\sqrt{n}(\bar{X}-\mu)}{\sigma}}} \\
     & =\E*{e^{\frac{t}{\sqrt{n}} \sum_{i=1}^{n} Y_i}}   \\
     & =\E*{\prod_{i=1}^n e^{\frac{t}{\sqrt{n}} Y_i}}    \\
     & =\prod_{i=1}^n\E*{e^{\frac{t}{\sqrt{n}} Y_i}}     \\
\end{align*}
Suppose $ Y_i $ has m.g.f.\ $ M_Y(t) $, then
\begin{itemize}
    \item $ M_Y(0)=1 $
    \item $ M_Y^\prime(0)=0 $
    \item $ M_Y^{\prime\prime}(0)=\E{Y^2}=\Var{Y}+(\E{Y})^2=1 $
\end{itemize}
\[ M_n(t)=\biggl[M_Y\biggl( \frac{t}{\sqrt{n}} \biggr)\biggr]^n \]
since $
    \displaystyle \E*{\expon*{\frac{t}{\sqrt{n}}Y_i}}=M_Y\biggl(\frac{t}{\sqrt{n}}\biggr) $
Step 2: We want to show that
\[ \lim\limits_{{n} \to {\infty}}
    \biggl[M_Y\biggl(\frac{t}{\sqrt{n}} \biggr)\biggr]^n=\expon*{\frac{t^2}{2}} \]
\begin{align*}
    M_Y\biggl(\frac{t}{\sqrt{n}} \biggr)
     & =M_Y(0)+M_Y^\prime(0)\biggl(\frac{t}{\sqrt{n}} \biggr)+
    \frac{M_Y^{\prime\prime}(0)}{2!}\biggl(\frac{t}{\sqrt{n}} \biggr)^2
    +o\biggl[\biggl(\frac{t}{\sqrt{n}} \biggr)^2\biggr]        \\
     & =1+\frac{t^2}{2n} +o\biggl(\frac{t^2}{n}\biggr)
\end{align*}
Then,
\[ \lim\limits_{{n} \to {\infty}}1+\frac{t^2}{2n} +o\biggl(\frac{t^2}{n}\biggr)=
    \lim\limits_{{n} \to {\infty}} \biggl(1+\frac{t^2}{2n}\biggr)=\expon*{\frac{t^2}{2}}  \]
\begin{Example}{}{}
    Suppose that $ X_1,\ldots,X_n \stackrel{\text{iid}}{\sim} \chi^2(1) $
    and $ Y_n=\sum_{i=1}^{n} X_i $. Show that
    \[ \frac{Y_n-n}{\sqrt{2n}} \stackrel{\text{d}}{\to}\N{0,1} \]
    \textbf{Solution.} $ \E{X_i}=1=\mu $ and $ \Var{X_i}=2=\sigma^2<\infty $.
    CLT tells us
    \[ \frac{\sqrt{n}(\bar{X}_n-\mu)}{\sigma}=
        \frac{\sqrt{n}(\bar{X}_n-1)}{\sqrt{2}}\stackrel{\text{d}}{\to}Z\sim \N{0,1} \]
    \[ \frac{Y_n-n}{\sqrt{2n}}=
        \frac{\sum_{i=1}^{n} X_i-n}{\sqrt{2n}}=\frac{n(\bar{X}_n-1)}{\sqrt{2n}}
        =\frac{\sqrt{n}(\bar{X}_n-1)}{\sqrt{2}}\stackrel{\text{d}}{\to}Z\sim\N{0,1}  \]
    Suppose that $ Y_n \sim \chi^2(n) $, we might ask you to prove
    \[ \frac{Y_n-n}{\sqrt{2n}} \stackrel{\text{d}}{\to}Z\sim \N{0,1} \]
    and you might have to figure out $ Y_n=\sum_{i=1}^{n} X_i $
    where $ X_1,\ldots,X_n\stackrel{\text{iid}}{\sim}\chi^2(1) $.
\end{Example}
\begin{Example}{}{}
    $ X_1,\ldots,X_n\stackrel{\text{iid}}{\sim}\poi{\mu} $.
    Let $ Y_n=\sum_{i=1}^{n} X_i $. Find the limiting
    distribution of $ \displaystyle \frac{Y_n-n\mu}{\sqrt{n\mu}} $.

    \textbf{Solution.} CLT tells us that
    \[ \frac{\sqrt{n}(\bar{X}_n-\mu)}{\sqrt{\mu}}\stackrel{\text{d}}{\to}Z\sim \N{0,1} \]
    Now,
    \[ \frac{Y_n-n\mu}{\sqrt{n\mu}}=
        \frac{\sum_{i=1}^{n} X_i-n\mu}{\sqrt{n\mu}}=
        \frac{n(\bar{X}_n-\mu)}{\sqrt{n\mu}}=
        \frac{\sqrt{n}(\bar{X}_n-\mu)}{\sqrt{\mu}}\stackrel{\text{d}}{\to}Z\sim \N{0,1}  \]
    Alternatively: If $ Y_n \sim \poi{n\mu} $, what is the limiting
    distribution of  $ \displaystyle \frac{Y_n-n\mu}{\sqrt{n\mu}} $?
\end{Example}
\begin{Theorem}{Continuous Mapping Theorem}{}
    Suppose that $ g(\cdot) $ is a continuous function.
    \begin{enumerate}[label=(\arabic*)]
        \item If $ X_n\stackrel{\mathbb{P}}{\to}a $, then
              $ g(X_n)\stackrel{\mathbb{P}}{\to}g(a) $.
        \item If $ X_n\stackrel{\text{d}}{\to}X $,
              then $ g(X_n)\stackrel{\text{d}}{\to}g(X) $.
    \end{enumerate}
\end{Theorem}
\begin{Theorem}{Slutsky's Theorem}{}
    If $ X_n\stackrel{\text{d}}{\to} X $, and
    $ Y_n\stackrel{\mathbb{P}}{\to}b $, then
    \begin{enumerate}[label=(\alph*)]
        \item $ X_n+Y_n\stackrel{\text{d}}{\to}X+b $.
              If we replace $ b $ by $ Y $ it is still true.
        \item $ X_n Y_n\stackrel{\text{d}}{\to}bX $.
        \item $ \displaystyle \frac{X_n}{Y_n}\stackrel{\text{d}}{\to}
                  \frac{X}{b} $ for $ b\neq 0 $.
    \end{enumerate}
\end{Theorem}
\begin{Exercise}{}{}
    Find a counter-example to the following statement.
    If $ X_n\stackrel{\text{d}}{\to}X $ and $ Y_n\stackrel{\text{d}}{\to}Y $,
    then
    \[ X_n+Y_n\stackrel{\text{d}}{\to}X+Y \]
\end{Exercise}
\begin{Example}{}{}
    If we have $ X_n\ge 0 $, $ a\ge 0 $,
    \begin{itemize}
        \item $ \sqrt{X_n}\stackrel{\mathbb{P}}{\to}\sqrt{a} $
        \item If $ X_n \stackrel{\mathbb{P}}{\to} a $, then
              $ X_n^2\stackrel{\mathbb{P}}{\to}a^2 $.
    \end{itemize}

    If $ X_n\stackrel{\text{d}}{\to}X \sim \N{0,1} $, then
    \begin{itemize}
        \item $ 2X_n\stackrel{\text{d}}{\to}2X\sim\N{0,4} $.
        \item $ 2X_n+1\stackrel{\text{d}}{\to}2X+1\sim\N{1,4} $.
        \item $ X_n^2\stackrel{\text{d}}{\to} X^2 \sim \chi^2(1) $.
    \end{itemize}

    If $ X_n\stackrel{\text{d}}{\to}X \sim \N{0,1} $
    and $ Y_n\stackrel{\mathbb{P}}{\to}b $ for $ b\neq 0 $, then
    \begin{itemize}
        \item $ X_n+Y_n\stackrel{\text{d}}{\to}X+b \sim \N{b,1} $.
        \item $ X_n Y_n \stackrel{\text{d}}{\to}bX \sim \N{0,b^2} $.
        \item $ \displaystyle \frac{X_n}{Yn} \stackrel{\text{d}}{\to}
                  \frac{X}{b}\sim \N*{0,\frac{1}{b^2}} $.
    \end{itemize}
\end{Example}
\begin{Example}{}{}
    Suppose that $ X_1,\ldots,X_n\stackrel{\text{iid}}{\sim}\poi{\mu} $.
    Find the limiting distribution of
    \[ Z_n=\frac{\sqrt{n}(\bar{X}_n-\mu)}{\sqrt{\bar{X}_n}}  \]
    \[ U_n=\sqrt{n}(\bar{X}_n-\mu) \]
    \textbf{Solution.} For $ Z_n $,
    \[ \frac{\sqrt{n}(\bar{X}_n-\mu)}{\sqrt{\mu}}\stackrel{\text{d}}{\to}Z
        \sim \N{0,1}  \]
    \[ Z_n=\frac{\sqrt{n}(\bar{X}_n-\mu)}{\sqrt{\bar{X}_n}}=
        \frac{\sqrt{n}(\bar{X}_n-\mu)}{\sqrt{\mu}}\cdot\frac{\sqrt{\mu}}{\sqrt{\bar{X}_n}}    \]
    By continuous mapping theorem,
    \[ \frac{\sqrt{\mu}}{\sqrt{\bar{X}_n}}\stackrel{\mathbb{P}}{\to}\frac{\sqrt{\mu}}{\sqrt{\mu}}=1
        \text{ since $ \bar{X}_n\stackrel{\mathbb{P}}{\to}\mu $ by WLLN} \]
    For $ U_n $, by Slutsky's theorem, $ Z_n\stackrel{\text{d}}{\to}Z \sim \N{0,1} $.
    \[ U_n=\sqrt{n}(\bar{X}_n-\mu)=\frac{\sqrt{n}(\bar{X}_n-\mu)}{\sqrt{\mu}}\sqrt{\mu}
        \stackrel{\text{d}}{\to}\sqrt{\mu}Z \sim \N{0,\mu}\text{ by
            continuous mapping theorem}  \]
\end{Example}
